Preservation for second UPc' query.

LR3_Compressed.thy
@@ -7,10 +7,18 @@ definition UPc :: \<open>(whole \<times> whole \<times> db) ell2 \<Rightarrow>\<
   (reg_1_3 o Fst; reg_2_3 o Snd) cnot o\<^sub>C\<^sub>L
   (reg_1_3 o Snd; reg_2_3 o Fst) cnot o\<^sub>C\<^sub>L
   (reg_1_3 o Fst; (reg_2_3 o Fst; reg_3_3)) query\<close>
+(* U_UP,i, using compressed queries, query' variant *)
+(* We probably will only use this one because we want to use preserve_query1'_fixY_output which is only available for query *)
+definition UPc' :: \<open>(whole \<times> whole \<times> db) ell2 \<Rightarrow>\<^sub>C\<^sub>L (whole \<times> whole \<times> db) ell2\<close> where \<open>UPc' = 
+  (reg_1_3 o Fst; reg_2_3 o Snd) cnot o\<^sub>C\<^sub>L
+  (reg_1_3 o Snd; reg_2_3 o Fst) cnot o\<^sub>C\<^sub>L
+  (reg_1_3 o Fst; (reg_2_3 o Fst; reg_3_3)) query'\<close>
 
 (* LR3 using compressed oracles *)
 definition LR3c where \<open>LR3c =
   (X;(X1;D1)) UPc o\<^sub>C\<^sub>L (X1;(X2;D2)) UPc o\<^sub>C\<^sub>L (X2;(Y;D3)) UPc o\<^sub>C\<^sub>L (X1;(X2;D2)) UPc o\<^sub>C\<^sub>L (X;(X1;D1)) UPc\<close>
+definition LR3c' where \<open>LR3c' =
+  (X;(X1;D1)) UPc' o\<^sub>C\<^sub>L (X1;(X2;D2)) UPc' o\<^sub>C\<^sub>L (X2;(Y;D3)) UPc' o\<^sub>C\<^sub>L (X1;(X2;D2)) UPc' o\<^sub>C\<^sub>L (X;(X1;D1)) UPc'\<close>
 
 (* Notion of good from the current eprint of the LR4-paper. Note: uniqueness condition missing. *)
 definition old_good where \<open>old_good D1 D2 D3 \<longleftrightarrow> (\<forall>x2L \<in> dom D3. \<exists>xL\<in>dom D1. \<exists>\<beta>\<in>ran D2. x2L = xL + \<beta>)\<close>
@@ -43,7 +51,7 @@ qed
 
 definition old_good_state_00 :: \<open>state set\<close> where \<open>old_good_state_00 = {(x,0,0,y,D1,D2,D3)| x y D1 D2 D3. old_good D1 D2 D3}\<close>
 definition old_good_state_0 :: \<open>state set\<close> where \<open>old_good_state_0 = {(x,x1,0,y,D1,D2,D3)| x x1 y D1 D2 D3. old_good D1 D2 D3}\<close>
-(* definition old_good_state :: \<open>state set\<close> where \<open>old_good_state = {(x,x1,x2,y,D1,D2,D3). old_good D1 D2 D3}\<close> *)
+definition old_good_state :: \<open>state set\<close> where \<open>old_good_state = {(x,x1,x2,y,D1,D2,D3). old_good D1 D2 D3}\<close>
 
 definition \<open>co1_old_good = 2 / sqrt N\<close>
 lemma preserves_co1_old_good:
@@ -147,6 +155,109 @@ proof -
   qed
 qed
 
+definition \<open>co1'_old_good = 2 / sqrt N\<close>
+lemma preserves_co1'_old_good:
+  \<open>preserves_ket ((X o Fst; (X1 o Fst; D1)) query') old_good_state_00 old_good_state_0 co1'_old_good\<close>
+proof -
+  define K :: \<open>(half\<times>half\<times>whole\<times>db\<times>db\<times>db) \<Rightarrow> state ell2 ccsubspace\<close> 
+    where \<open>K = (\<lambda>(xL,xR,y,D1',D2,D3).
+          ket_invariant {((xL,xR),(x1L,0),0,y,D1'(xL:=d),D2,D3) | x1L d. True})\<close>
+  define M :: \<open>(half\<times>half\<times>whole\<times>db\<times>db\<times>db) set\<close> where
+    \<open>M = {(xL,xR,y,D1',D2,D3). D1' xL = None \<and> (\<exists>d. old_good (D1'(xL:=d)) D2 D3)}\<close>
+
+  define I1 J1 :: \<open>(half\<times>half\<times>whole\<times>db\<times>db\<times>db) \<Rightarrow> (half \<times> half option) set\<close> 
+    where \<open>I1 = (\<lambda>(xL,xR,y,D1',D2,D3).
+          {0} \<times> {d. old_good (D1'(xL:=d)) D2 D3})\<close>
+      and \<open>J1 = (\<lambda>(xL,xR,y,D1',D2,D3). 
+          UNIV \<times> {d. old_good (D1'(xL:=d)) D2 D3})\<close>
+
+  show ?thesis
+  proof (rule inv_split_reg_query'[where X=\<open>X o Fst\<close> and Y=\<open>X1 o Fst\<close> and H=\<open>D1\<close> and K=K
+        and ?I1.0=\<open>\<lambda>z. ket_invariant (I1 z)\<close> and ?J1.0=\<open>\<lambda>z. ket_invariant (J1 z)\<close>])
+    show \<open>(X \<circ> Fst;(X1 \<circ> Fst;D1)) query' = (X \<circ> Fst;(X1 \<circ> Fst;D1)) query'\<close>
+      by simp
+    show [simp]: \<open>compatible (X \<circ> Fst) (X1 \<circ> Fst)\<close> \<open>compatible (X \<circ> Fst) D1\<close> \<open>compatible (X1 \<circ> Fst) D1\<close>
+      by simp_all
+    show \<open>compatible_register_invariant (X1 \<circ> Fst) (K z)\<close> for z
+      apply (cases z, hypsubst_thin)
+      by (auto simp add: K_def X1_def comp_assoc
+          intro!: compatible_register_invariant_Snd_comp compatible_register_invariant_Fst compatible_register_invariant_Fst_comp)
+    show \<open>compatible_register_invariant (D1 \<circ> function_at (fst z)) (K z)\<close> for z
+      by (auto simp add: K_def D1_def comp_assoc case_prod_beta
+          intro!: compatible_register_invariant_Snd_comp compatible_register_invariant_Fst compatible_register_invariant_Fst_comp
+          compatible_register_invariant_function_at)
+    show \<open>ket_invariant old_good_state_00 \<le> (SUP z\<in>M. K z \<sqinter> lift_invariant (X1 \<circ> Fst;D1 \<circ> function_at (fst z)) (ket_invariant (I1 z)))\<close>
+      apply (auto simp add: K_def D1_def lift_Fst_ket_inv ket_invariant_inter ket_invariant_SUP[symmetric] I1_def
+          old_good_state_00_def case_prod_beta comp_assoc X1_def M_def zero_prod_def
+          lift_inv_prod lift_invariant_comp lift_invariant_function_at_ket_inv lift_Snd_ket_inv)
+      by (metis fun_upd_same fun_upd_triv fun_upd_upd)
+    show \<open>K z \<sqinter> lift_invariant (X1 \<circ> Fst;D1 \<circ> function_at (fst z)) (ket_invariant (J1 z)) \<le> ket_invariant old_good_state_0\<close>
+      if \<open>z\<in>M\<close> for z
+      using that 
+      apply (cases z, hypsubst_thin)
+      by (auto simp add: K_def lift_Fst_ket_inv ket_invariant_inter ket_invariant_SUP[symmetric] J1_def
+          case_prod_beta D1_def comp_assoc X1_def old_good_state_0_def M_def
+          lift_inv_prod lift_invariant_comp lift_invariant_function_at_ket_inv reg_3_3_def lift_Snd_ket_inv)
+    show \<open>orthogonal_spaces (K z) (K z')\<close> if \<open>z\<in>M\<close> \<open>z'\<in>M\<close> \<open>z \<noteq> z'\<close> for z z'
+      apply (cases z; cases z')
+      using that apply (auto simp: K_def M_def)
+      by (metis fun_upd_triv fun_upd_upd)
+    show \<open>K z \<le> lift_invariant (X \<circ> Fst) (ket_invariant {fst z})\<close> for z
+      by (auto simp: K_def X_def lift_Fst_ket_inv lift_invariant_comp case_prod_beta)
+    show [simp]: \<open>0 \<le> co1'_old_good\<close>
+      by (simp add: co1'_old_good_def)
+    show \<open>preserves_ket query1' (I1 z) (J1 z) co1'_old_good\<close> if \<open>z\<in>M\<close> for z
+    proof (cases z)
+      case (fields xL xR y D1' D2 D3)
+      from that have D1'xL: \<open>D1' xL = None\<close>
+        by (auto simp: M_def fields)
+      show ?thesis
+      proof (cases \<open>old_good D1' D2 D3\<close>)
+        case True
+        show ?thesis
+          apply (simp only: case_prod_beta I1_def J1_def fst_conv snd_conv fields)
+        proof (rule preserve_query1'_fixY[where b\<^sub>i=N and b\<^sub>j\<^sub>0=0])
+          show \<open>{d. old_good (D1'(xL := d)) D2 D3} \<subseteq> {d. old_good (D1'(xL := d)) D2 D3}\<close> by simp
+          show \<open>card (Some -` {d. old_good (D1'(xL := d)) D2 D3}) \<le> N\<close> by (simp add: card_mono)
+          show \<open>card (- Some -` {d. old_good (D1'(xL := d)) D2 D3}) \<le> 0\<close> 
+            using True D1'xL apply auto
+            by (simp add: old_good_def)
+          have *: \<open>old_good (D1'(xL := None)) D2 D3\<close>
+            by (simp add: D1'xL True domIff)
+          show \<open>co1'_old_good \<ge> 0\<close>
+            by simp
+          then show \<open>preserve_query1'_fixY_bound
+             (None \<in> {d. old_good (D1'(xL := d)) D2 D3}) (None \<notin> {d. old_good (D1'(xL := d)) D2 D3})
+             (real N) (real 0) \<le> co1'_old_good\<close>
+            by (simp add: * preserve_query1'_fixY_bound_def)
+        qed
+      next
+        case False
+        show ?thesis
+          apply (simp only: case_prod_beta I1_def J1_def fst_conv snd_conv fields)
+        proof (rule preserve_query1'_fixY[where b\<^sub>i=N and b\<^sub>j\<^sub>0=0])
+          show \<open>{d. old_good (D1'(xL := d)) D2 D3} \<subseteq> {d. old_good (D1'(xL := d)) D2 D3}\<close> by simp
+          show \<open>card (Some -` {d. old_good (D1'(xL := d)) D2 D3}) \<le> N\<close>
+            by (simp add: card_mono)
+          show \<open>card (- Some -` {d. old_good (D1'(xL := d)) D2 D3}) \<le> 0\<close>
+            using False \<open>z\<in>M\<close>
+            apply (auto simp: M_def fields old_good_def)
+            by (metis DiffE domI insert_iff)
+          have *: \<open>\<not> old_good (D1'(xL := None)) D2 D3\<close>
+            by (simp add: D1'xL False domIff)
+          show \<open>preserve_query1'_fixY_bound (None \<in> {d. old_good (D1'(xL := d)) D2 D3}) (None \<notin> {d. old_good (D1'(xL := d)) D2 D3})
+                     (real N) (real 0) \<le> co1'_old_good\<close>
+            apply (auto simp add: * preserve_query1'_fixY_bound_def co1'_old_good_def)
+            by (simp add: inverse_eq_divide sqrt_divide_self_eq)
+          show \<open>0 \<le> co1'_old_good\<close>
+            by simp
+        qed
+      qed
+    qed
+  qed
+qed
+
+
 definition \<open>UPc1_old_good = co1_old_good\<close>
 lemma preserves_UPc1_old_good:
   \<open>preserves_ket ((X;(X1;D1)) UPc) old_good_state_00 old_good_state_0 UPc1_old_good\<close>
@@ -175,4 +286,195 @@ proof -
     by (auto simp add: UPc1_old_good_def UPc cblinfun_compose_assoc register_norm)
 qed
 
+definition \<open>UPc1'_old_good = co1'_old_good\<close>
+lemma preserves_UPc1'_old_good:
+  \<open>preserves_ket ((X;(X1;D1)) UPc') old_good_state_00 old_good_state_0 UPc1'_old_good\<close>
+proof -
+  note comp_apply[simp del]
+
+  have UPc: \<open>((X;(X1;D1)) UPc') = 
+      (X o Fst; X1 o Snd) cnot o\<^sub>C\<^sub>L (X \<circ> Snd; X1 \<circ> Fst) cnot o\<^sub>C\<^sub>L (X \<circ> Fst; (X1 \<circ> Fst; D1)) query'\<close>
+    by (simp add: UPc'_def reg_1_3_def reg_2_3_def reg_3_3_def register_pair_Fst register_pair_Snd
+        flip: register_mult comp_assoc register_comp_pair 
+        o_apply[where x=cnot and f=\<open>(X;(X1;D1))\<close>] o_apply[where x=query' and f=\<open>(X;(X1;D1))\<close>])
+
+  have \<open>preserves_ket ((X \<circ> Fst; (X1 \<circ> Fst; D1)) query') old_good_state_00 old_good_state_0 co1'_old_good\<close>
+    by (rule preserves_co1'_old_good)
+  also have \<open>preserves_ket ((X \<circ> Snd; X1 \<circ> Fst) cnot) old_good_state_0 old_good_state_0 0\<close>
+    apply (rule preserves_compatible[where U=cnot])
+    by (auto simp add: old_good_state_0_def X_def X1_def comp_assoc
+        intro!: compatible_register_invariant_pair compatible_register_invariant_Fst_comp
+        compatible_register_invariant_Snd_comp)
+  also have \<open>preserves_ket ((X \<circ> Fst; X1 \<circ> Snd) cnot) old_good_state_0 old_good_state_0 0\<close>
+    apply (rule preserves_compatible[where U=cnot])
+    by (auto simp add: old_good_state_0_def X_def X1_def comp_assoc
+        intro!: compatible_register_invariant_pair compatible_register_invariant_Fst_comp
+        compatible_register_invariant_Snd_comp)
+  finally show ?thesis
+    by (auto simp add: UPc1'_old_good_def UPc cblinfun_compose_assoc register_norm)
+qed
+
+definition num_queries_D1 :: \<open>nat \<Rightarrow> state set\<close> where \<open>num_queries_D1 q = {(x,x1,x2,y,D1,D2,D3). card (dom D1) \<le> q}\<close>
+
+(* TODO: preservation lemma for num_queries_1 *)
+
+definition \<open>co2'_old_good q = 2 * sqrt q / N  +  2 * sqrt q / sqrt N  +  1 / sqrt N\<close>
+lemma preserves_co2'_old_good:
+  \<open>preserves_ket ((X1 o Fst; (X2 o Fst; D2)) query') (old_good_state_0 \<inter> num_queries_D1 q) old_good_state (co2'_old_good q)\<close>
+proof -
+  define K :: \<open>(half\<times>half\<times>whole\<times>whole\<times>db\<times>db\<times>db) \<Rightarrow> state ell2 ccsubspace\<close> 
+    where \<open>K = (\<lambda>(x1L,x1R,x,y,D1,D2',D3).
+          ket_invariant {(x,(x1L,x1R),(x2L,0),y,D1,D2'(x1L:=d),D3) | x2L d. True})\<close>
+  define M :: \<open>(half\<times>half\<times>whole\<times>whole\<times>db\<times>db\<times>db) set\<close> where
+    \<open>M = {(x1L,x1R,x,y,D1,D2',D3). D2' x1L = None \<and> (\<exists>d. old_good D1 (D2'(x1L:=d)) D3) \<and> card (dom D1) \<le> q}\<close>
+
+  define I1 J1 :: \<open>(half\<times>half\<times>whole\<times>whole\<times>db\<times>db\<times>db) \<Rightarrow> (half \<times> half option) set\<close> 
+    where \<open>I1 = (\<lambda>(x1L,x1R,x,y,D1,D2',D3).
+          {0} \<times> {d. old_good D1 (D2'(x1L:=d)) D3})\<close>
+      and \<open>J1 = (\<lambda>(x1L,x1R,x,y,D1,D2',D3).
+          UNIV \<times> {d. old_good D1 (D2'(x1L:=d)) D3})\<close>
+
+  show ?thesis
+  proof (rule inv_split_reg_query'[where X=\<open>X1 o Fst\<close> and Y=\<open>X2 o Fst\<close> and H=\<open>D2\<close> and K=K
+        and ?I1.0=\<open>\<lambda>z. ket_invariant (I1 z)\<close> and ?J1.0=\<open>\<lambda>z. ket_invariant (J1 z)\<close>])
+    show \<open>(X1 \<circ> Fst;(X2 \<circ> Fst;D2)) query' = (X1 \<circ> Fst;(X2 \<circ> Fst;D2)) query'\<close>
+      by simp
+    show [simp]: \<open>compatible (X1 \<circ> Fst) (X2 \<circ> Fst)\<close> \<open>compatible (X1 \<circ> Fst) D2\<close> \<open>compatible (X2 \<circ> Fst) D2\<close>
+      by simp_all
+    show \<open>compatible_register_invariant (X2 \<circ> Fst) (K z)\<close> for z
+      apply (cases z, hypsubst_thin)
+      by (auto simp add: K_def X2_def comp_assoc
+          intro!: compatible_register_invariant_Snd_comp compatible_register_invariant_Fst compatible_register_invariant_Fst_comp)
+    show \<open>compatible_register_invariant (D2 \<circ> function_at (fst z)) (K z)\<close> for z
+      by (auto simp add: K_def D2_def comp_assoc case_prod_beta
+          intro!: compatible_register_invariant_Snd_comp compatible_register_invariant_Fst compatible_register_invariant_Fst_comp
+          compatible_register_invariant_function_at)
+    show \<open>ket_invariant (old_good_state_0 \<inter> num_queries_D1 q) \<le> (SUP z\<in>M. K z \<sqinter> lift_invariant (X2 \<circ> Fst;D2 \<circ> function_at (fst z)) (ket_invariant (I1 z)))\<close>
+      apply (auto simp add: K_def D2_def lift_Fst_ket_inv ket_invariant_inter ket_invariant_SUP[symmetric] I1_def
+          old_good_state_0_def case_prod_beta comp_assoc X2_def M_def zero_prod_def num_queries_D1_def
+          lift_inv_prod lift_invariant_comp lift_invariant_function_at_ket_inv lift_Snd_ket_inv)
+      by (metis fun_upd_same fun_upd_triv fun_upd_upd)
+    show \<open>K z \<sqinter> lift_invariant (X2 \<circ> Fst;D2 \<circ> function_at (fst z)) (ket_invariant (J1 z)) \<le> ket_invariant old_good_state\<close>
+      if \<open>z\<in>M\<close> for z
+      using that 
+      apply (cases z, hypsubst_thin)
+      by (auto simp add: K_def lift_Fst_ket_inv ket_invariant_inter ket_invariant_SUP[symmetric] J1_def
+          case_prod_beta D2_def comp_assoc X2_def old_good_state_def M_def
+          lift_inv_prod lift_invariant_comp lift_invariant_function_at_ket_inv reg_3_3_def lift_Snd_ket_inv)
+    show \<open>orthogonal_spaces (K z) (K z')\<close> if \<open>z\<in>M\<close> \<open>z'\<in>M\<close> \<open>z \<noteq> z'\<close> for z z'
+      apply (cases z; cases z')
+      using that apply (auto simp: K_def M_def)
+      by (metis fun_upd_triv fun_upd_upd)
+    show \<open>K z \<le> lift_invariant (X1 \<circ> Fst) (ket_invariant {fst z})\<close> for z
+      by (auto simp: K_def X1_def lift_Fst_ket_inv lift_Snd_ket_inv lift_invariant_comp case_prod_beta)
+    show [simp]: \<open>0 \<le> co2'_old_good q\<close>
+      by (simp add: co2'_old_good_def)
+    show \<open>preserves_ket query1' (I1 z) (J1 z) (co2'_old_good q)\<close> if \<open>z\<in>M\<close> for z
+    proof (cases z)
+      case (fields x1L x1R x y D1 D2' D3)
+      from that have D2'xL: \<open>D2' x1L = None\<close>
+        by (auto simp: M_def fields)
+      show ?thesis
+      proof (cases \<open>old_good D1 D2' D3\<close>)
+        case True
+        show ?thesis
+          apply (simp only: case_prod_beta I1_def J1_def fst_conv snd_conv fields)
+        proof (rule preserve_query1'_fixY[where b\<^sub>i=N and b\<^sub>j\<^sub>0=0])
+          show \<open>{d. old_good D1 (D2'(x1L := d)) D3} \<subseteq> {d. old_good D1 (D2'(x1L := d)) D3}\<close> by simp
+          show \<open>card (Some -` {d. old_good D1 (D2'(x1L := d)) D3}) \<le> N\<close> by (simp add: card_mono)
+          show \<open>card (- Some -` {d. old_good D1 (D2'(x1L := d)) D3}) \<le> 0\<close>
+            using True D2'xL apply auto
+            apply (simp add: old_good_def)
+            by meson
+          have *: \<open>old_good D1 (D2'(x1L := None)) D3\<close>
+            by (simp add: D2'xL True domIff)
+          show \<open>co2'_old_good q \<ge> 0\<close>
+            by simp
+          then show \<open>preserve_query1'_fixY_bound
+             (None \<in> {d. old_good D1 (D2'(x1L := d)) D3}) (None \<notin> {d. old_good D1 (D2'(x1L := d)) D3})
+             (real N) (real 0) \<le> (co2'_old_good q)\<close>
+            by (simp add: * preserve_query1'_fixY_bound_def)
+        qed
+      next
+        case False
+        show ?thesis
+          apply (simp only: case_prod_beta I1_def J1_def fst_conv snd_conv fields)
+        proof (rule preserve_query1'_fixY[where b\<^sub>i=q and b\<^sub>j\<^sub>0=N])
+          show \<open>{d. old_good D1 (D2'(x1L := d)) D3} \<subseteq> {d. old_good D1 (D2'(x1L := d)) D3}\<close> by simp
+          have card_D1: \<open>card (dom D1) \<le> q\<close>
+            using \<open>z\<in>M\<close> by (simp add: fields M_def)
+          from False obtain x2L where \<open>x2L \<in> dom D3\<close> and x2L_not_good: \<open>\<forall>xL\<in>dom D1. \<forall>\<beta>\<in>ran D2'. x2L \<noteq> xL + \<beta>\<close>
+            by (auto simp: old_good_def)
+          have d_poss: \<open>Some -` {d. old_good D1 (D2'(x1L := d)) D3} \<subseteq> (+) x2L ` dom D1\<close>
+          proof (rule subsetI, rename_tac d)
+            fix d assume \<open>d \<in> Some -` {d. old_good D1 (D2'(x1L := d)) D3}\<close>
+            then have \<open>old_good D1 (D2'(x1L \<mapsto> d)) D3\<close>
+              by simp
+            with \<open>x2L \<in> dom D3\<close> have \<open>\<exists>xL\<in>dom D1. \<exists>\<beta>\<in>ran (D2'(x1L \<mapsto> d)). x2L = xL + \<beta>\<close>
+              by (simp add: old_good_def)
+            with x2L_not_good have \<open>\<exists>xL\<in>dom D1. x2L = xL + d\<close>
+              using D2'xL by auto
+            then show \<open>d \<in> (+) x2L ` dom D1\<close>
+              by force
+          qed
+          show \<open>card (Some -` {d. old_good D1 (D2'(x1L := d)) D3}) \<le> q\<close>
+            using _ card_D1 apply (rule order.trans)
+            using d_poss by (simp add: surj_card_le)
+          show \<open>card (- Some -` {d. old_good D1 (D2'(x1L := d)) D3}) \<le> N\<close>
+            by (simp add: card_mono)
+          have *: \<open>\<not> old_good D1 (D2'(x1L := None)) D3\<close>
+            by (simp add: D2'xL False domIff)
+          show \<open>preserve_query1'_fixY_bound (None \<in> {d. old_good D1 (D2'(x1L := d)) D3}) (None \<notin> {d. old_good D1 (D2'(x1L := d)) D3})
+                     (real q) (real N) \<le> co2'_old_good q\<close>
+            apply (auto simp add: * preserve_query1'_fixY_bound_def co2'_old_good_def)
+            by (metis ab_semigroup_mult_class.mult_ac(1) dual_order.refl of_nat_0_le_iff real_divide_square_eq sqrt_sqrt times_divide_eq_right)
+          show \<open>0 \<le> co2'_old_good q\<close>
+            by simp
+        qed
+      qed
+    qed
+  qed
+qed
+
+
+definition \<open>UPc2'_old_good q = co2'_old_good q\<close>
+lemma preserves_UPc2'_old_good:
+  \<open>preserves_ket ((X1;(X2;D2)) UPc') (old_good_state_0 \<inter> num_queries_D1 q) old_good_state (UPc2'_old_good q)\<close>
+proof -
+  note comp_apply[simp del]
+
+  have UPc: \<open>((X1;(X2;D2)) UPc') = 
+      (X1 o Fst; X2 o Snd) cnot o\<^sub>C\<^sub>L (X1 \<circ> Snd; X2 \<circ> Fst) cnot o\<^sub>C\<^sub>L (X1 \<circ> Fst; (X2 \<circ> Fst; D2)) query'\<close>
+    by (simp add: UPc'_def reg_1_3_def reg_2_3_def reg_3_3_def register_pair_Fst register_pair_Snd
+        flip: register_mult comp_assoc register_comp_pair 
+        o_apply[where x=cnot and f=\<open>(X1;(X2;D2))\<close>] o_apply[where x=query' and f=\<open>(X1;(X2;D2))\<close>])
+
+  have \<open>preserves_ket ((X1 \<circ> Fst; (X2 \<circ> Fst; D2)) query') (old_good_state_0 \<inter> num_queries_D1 q) old_good_state (co2'_old_good q)\<close>
+    by (rule preserves_co2'_old_good)
+  also have \<open>preserves_ket ((X1 \<circ> Snd; X2 \<circ> Fst) cnot) old_good_state old_good_state 0\<close>
+    apply (rule preserves_compatible[where U=cnot])
+    by (auto simp add: old_good_state_def X1_def X2_def comp_assoc
+        intro!: compatible_register_invariant_pair compatible_register_invariant_Fst_comp
+        compatible_register_invariant_Snd_comp)
+  also have \<open>preserves_ket ((X1 \<circ> Fst; X2 \<circ> Snd) cnot) old_good_state old_good_state 0\<close>
+    apply (rule preserves_compatible[where U=cnot])
+    by (auto simp add: old_good_state_def X1_def X2_def comp_assoc
+        intro!: compatible_register_invariant_pair compatible_register_invariant_Fst_comp
+        compatible_register_invariant_Snd_comp)
+  finally show ?thesis
+    by (auto simp add: UPc2'_old_good_def UPc cblinfun_compose_assoc register_norm)
+qed
+
 end
+
+(* What we have so far:
+
+UPc1': old_good_state_00 \<longrightarrow> old_good_state_0
+UPc2': old_good_state_0 \<inter> num_queries_1 q \<longrightarrow> old_good_state
+
+Plugging this together with other stuff:
+UPc1';UPc2': old_good_state_00 \<inter> num_queries_1 q \<inter> num_queries_2 q 
+        \<longrightarrow>  old_good_state_00 \<inter> num_queries_1 (q+1) \<inter> num_queries_2 (q+1)
+             \<inter> x1,x2 have the right stuff given x,D1,D2
+
+*)
